src/extensions/paths/OperationalSemantics.v
@@ -6,6 +6,8 @@ Require Import Definitions Binding.
 
 (** * Stack-Based Operational Semantics *)
 
+Reserved Notation "t1 '|->' t2" (at level 40, t2 at level 39).
+
 Inductive red : sta * trm -> sta * trm -> Prop :=
 
 (** [s ∋ (p, lambda(T)t)  ]      #<br>#
@@ -13,15 +15,15 @@ Inductive red : sta * trm -> sta * trm -> Prop :=
     [(s, p q) |-> (s, t^q)]      *)
 | red_app: forall s p q T t,
     s ∋ (p, val_lambda T t) ->
-    (s, trm_app p q) |-> (s, open_trm_p p t)
+    (s, trm_app p q) |-> (s, open_trm_p q t)
 
 (** [(s, let x = v in t) |-> ((s, x = v), t^x)] *)
-| red_let : forall v t s x,
+| red_let_val : forall v t s x,
     x # s ->
     (s, trm_let (trm_val v) t) |-> (s & x ~ v, open_trm x t)
 
 (** [(s, let y = p in t) |-> (s, t^p)] *)
-| red_let_var : forall t s p,
+| red_let_path : forall t s p,
     (s, trm_let (trm_path p) t) |-> (s, open_trm_p p t)
 
 (** [(s, t0) |-> (s', t0')]                            #<br>#
